tests/elab/transport.lean
@@ -134,7 +134,7 @@ instance : Pointed Opt2 := by transport (Pointed Option)
 
 example : Pointed.point (m := Opt2) Nat 1 = Opt2.mk (Opt.mk (some 1)) := rfl
 
--- `MonadLift.congr` transports the target monad of a lift.
+-- `MonadLift.canonicalCongr` transports the target monad of a lift.
 instance : MonadLift Id Option := ⟨fun x => some x.run⟩
 
 instance : MonadLift Id Opt := inferInstanceAs (MonadLift Id Option)
